src/lib/communication/DY.Lib.Communication.RequestResponse.Properties.fst
@@ -10,8 +10,10 @@ open DY.Lib.State.PrivateKeys
 open DY.Lib.State.Typed
 
 open DY.Lib.Communication.Data
+open DY.Lib.Communication.Core
 open DY.Lib.Communication.RequestResponse
 open DY.Lib.Communication.RequestResponse.Invariants
+open DY.Lib.Communication.RequestResponse.Lemmas
 
 #set-options "--fuel 0 --ifuel 0 --z3rlimit 10 --z3cliopt 'smt.qi.eager_threshold=100'"
 
@@ -25,19 +27,19 @@ val server_authentication:
   #a:Type -> {| comm_layer_reqres_config a |} ->
   tr:trace -> i:timestamp ->
   higher_layer_resreq_preds:comm_reqres_higher_layer_event_preds a ->
-  client:principal -> server:principal -> response:a -> key:bytes ->
+  client:principal -> server:principal -> request:a -> response:a -> key:bytes ->
   Lemma
   (requires
     trace_invariant tr /\
     has_communication_layer_reqres_event_predicates higher_layer_resreq_preds /\
-    event_triggered_at tr i client (CommClientReceiveResponse client server  response key <: communication_reqres_event a)
+    event_triggered_at tr i client (CommClientReceiveResponse client server request response key <: communication_reqres_event a)
   )
   (ensures
     (exists request. event_triggered (prefix tr i) server (CommServerSendResponse server request response key <: communication_reqres_event a)) \/
     is_corrupt (prefix tr i) (principal_label client) \/
     is_corrupt (prefix tr i) (principal_label server)
   )
-let server_authentication #tag #invs #a tr i higher_layer_resreq_preds client server response key = ()
+let server_authentication #tag #invs #a tr i higher_layer_resreq_preds client server request response key = ()
 
 
 (*** Secrecy Security Property ***)
@@ -67,43 +69,63 @@ let key_secrecy_client #tag #invs tr client server key request response =
 
 (*** Properties ***)
 
+val derive_comm_client_state_invariant:
+  {|protocol_invariants|} ->
+  #a:Type -> {|comm_layer_reqres_config a|} ->
+  tr:trace ->
+  higher_layer_preds:comm_reqres_higher_layer_event_preds a ->
+  client:principal -> req_meta_data:comm_meta_data a ->
+  Lemma
+  (requires
+    trace_invariant tr /\
+    has_communication_layer_reqres_predicates higher_layer_preds /\
+    event_triggered tr client (CommClientSendRequest client req_meta_data.server req_meta_data.request req_meta_data.key <: communication_reqres_event a)
+  )
+  (ensures
+    is_knowable_by (principal_label client) tr req_meta_data.key /\
+    is_well_formed a (is_knowable_by (principal_label client) tr) req_meta_data.request
+  )
+let derive_comm_client_state_invariant #invs #a tr higher_layer_preds client req_meta_data = ()
+
 val request_message_properties:
   {|protocol_invariants|} ->
   #a:Type -> {|comm_layer_reqres_config a|} ->
   tr:trace -> i:timestamp ->
   higher_layer_preds:comm_reqres_higher_layer_event_preds a ->
-  server:principal -> key:bytes -> request:a ->
+  req_meta_data:comm_meta_data a ->
   Lemma
   (requires
     trace_invariant tr /\
     has_communication_layer_reqres_predicates higher_layer_preds /\
-    event_triggered_at tr i server (CommServerReceiveRequest server request key <: communication_reqres_event a)
+    event_triggered_at tr i req_meta_data.server (CommServerReceiveRequest req_meta_data.server req_meta_data.request req_meta_data.key <: communication_reqres_event a)
   )
   (ensures
-    is_well_formed a (is_knowable_by (principal_label server) (prefix tr i)) request /\
-    (exists client. higher_layer_preds.send_request (prefix tr i) client server request (get_label (prefix tr i) key)) \/
-    is_publishable (prefix tr i) key
+    is_well_formed a (is_knowable_by (principal_label req_meta_data.server) tr) req_meta_data.request /\
+    is_well_formed a (is_knowable_by (get_response_label tr req_meta_data) tr) req_meta_data.request /\
+    ((exists client. higher_layer_preds.send_request tr client req_meta_data.server req_meta_data.request (get_label tr req_meta_data.key)) \/
+    is_publishable tr req_meta_data.key)
   )
-let request_message_properties #invs #a tr i higher_layer_preds server key request =
-  let send_event client:communication_reqres_event a = CommClientSendRequest client server request key in
+let request_message_properties #invs #a tr i higher_layer_preds req_meta_data =
+  let send_event client:communication_reqres_event a = CommClientSendRequest client req_meta_data.server req_meta_data.request req_meta_data.key in
   let tr_i = prefix tr i in
-  let key_label = get_label tr_i key in
-  assert(is_well_formed a (is_knowable_by (principal_label server) tr_i) request);
+  let key_label = get_label tr_i req_meta_data.key in
+  get_response_label_eq_key_label tr req_meta_data;
+  assert(is_well_formed a (is_knowable_by (principal_label req_meta_data.server) tr_i) req_meta_data.request);
   assert(exists client. event_triggered tr_i client (send_event client) \/
-            is_publishable tr_i key);
+            is_publishable tr_i req_meta_data.key);
   eliminate (exists client. event_triggered tr_i client (send_event client)) \/
-            is_publishable tr_i key
+            is_publishable tr_i req_meta_data.key
   returns
-    is_well_formed a (is_knowable_by (principal_label server) tr_i) request /\
-    (exists client. higher_layer_preds.send_request tr_i client server request key_label) \/
-    is_publishable tr_i key
+    is_well_formed a (is_knowable_by (principal_label req_meta_data.server) tr) req_meta_data.request /\
+    (exists client. higher_layer_preds.send_request tr client req_meta_data.server req_meta_data.request key_label) \/
+    is_publishable tr req_meta_data.key
   with _. eliminate exists client. event_triggered tr_i client (send_event client)
     returns _
     with _. (
       let j = find_event_triggered_at_timestamp tr client (send_event client) in
       find_event_triggered_at_timestamp_later tr_i tr client (send_event client);
 
-      higher_layer_preds.send_request_later (prefix tr j) tr_i client server request key_label;
+      higher_layer_preds.send_request_later (prefix tr j) tr client req_meta_data.server req_meta_data.request key_label;
       ()
     )
   and _. ()
@@ -114,41 +136,47 @@ val response_message_properties:
   #a:Type -> {|comm_layer_reqres_config a|} ->
   tr:trace -> i:timestamp ->
   higher_layer_preds:comm_reqres_higher_layer_event_preds a ->
-  client:principal -> server:principal -> response:a -> req_meta_data:comm_meta_data a ->
+  client:principal -> response:a -> req_meta_data:comm_meta_data a ->
   Lemma
   (requires
     trace_invariant tr /\
     has_communication_layer_reqres_predicates higher_layer_preds /\
-    event_triggered_at tr i client (CommClientReceiveResponse client server response req_meta_data.key <: communication_reqres_event a)
+    event_triggered tr client (CommClientSendRequest client req_meta_data.server req_meta_data.request req_meta_data.key <: communication_reqres_event a) /\
+    event_triggered_at tr i client (CommClientReceiveResponse client req_meta_data.server req_meta_data.request response req_meta_data.key <: communication_reqres_event a)
   )
   (ensures
-    //is_well_formed a (is_knowable_by (principal_label client) (prefix tr i)) response /\
-    (exists request. higher_layer_preds.send_response tr server request response (get_label tr req_meta_data.key)) \/
-    is_corrupt tr (principal_label client) \/ is_corrupt tr (principal_label server)
+    is_well_formed a (is_knowable_by (comm_label client req_meta_data.server) tr) response /\
+    higher_layer_preds.send_request tr client req_meta_data.server req_meta_data.request (get_label tr req_meta_data.key) /\
+    ( 
+      higher_layer_preds.send_response tr req_meta_data.server req_meta_data.request response (get_label tr req_meta_data.key)
+    ) \/ (
+      is_corrupt tr (principal_label client) \/ is_corrupt tr (principal_label req_meta_data.server)
+    )
   )
-let response_message_properties #invs #a tr i higher_layer_preds client server response req_meta_data =
-  let send_event request:communication_reqres_event a = CommServerSendResponse server request response req_meta_data.key in
+let response_message_properties #invs #a tr i higher_layer_preds client response req_meta_data =
+  let send_event:communication_reqres_event a = CommServerSendResponse req_meta_data.server req_meta_data.request response req_meta_data.key in
   let tr_i = prefix tr i in
   let key_label = get_label tr req_meta_data.key in
-  //assert(is_well_formed a (is_knowable_by (principal_label client) tr_i) response);
-  assert((exists request. event_triggered tr_i server (send_event request)) \/
-            is_corrupt tr (principal_label client) \/ is_corrupt tr (principal_label server));
-  eliminate (exists request. event_triggered tr_i server (send_event request)) \/
-            (is_corrupt tr (principal_label client) \/ is_corrupt tr (principal_label server))
+
+  assert(is_well_formed a (is_knowable_by (comm_label client req_meta_data.server) tr) response);
+
+  let j' = find_event_triggered_at_timestamp tr client (CommClientSendRequest client req_meta_data.server req_meta_data.request req_meta_data.key <: communication_reqres_event a) in
+  assert(higher_layer_preds.send_request (prefix tr j') client req_meta_data.server req_meta_data.request (get_label (prefix tr j') req_meta_data.key));
+  higher_layer_preds.send_request_later (prefix tr j') tr client req_meta_data.server req_meta_data.request (get_label (prefix tr j') req_meta_data.key);
+
+  eliminate (event_triggered tr_i req_meta_data.server send_event) \/
+            (is_corrupt tr (principal_label client) \/ is_corrupt tr (principal_label req_meta_data.server))
   returns
-    //is_well_formed a (is_knowable_by (principal_label server) tr_i) response /\
-    (exists request. higher_layer_preds.send_response tr server request response key_label) \/
-      (is_corrupt tr (principal_label client) \/ is_corrupt tr (principal_label server))
-  with _. (
-    assert(exists request. event_triggered tr_i server (send_event request));
-    eliminate exists request. event_triggered tr_i server (send_event request)
-    returns exists request. higher_layer_preds.send_response tr server request response key_label
-    with _. (
-      let j = find_event_triggered_at_timestamp tr server (send_event request) in
-      find_event_triggered_at_timestamp_later tr_i tr server (send_event request);
-      get_label_later (prefix tr j) tr req_meta_data.key;
-      higher_layer_preds.send_response_later (prefix tr j) tr server request response key_label;
-      ()
+    is_well_formed a (is_knowable_by (principal_label req_meta_data.server) tr_i) response /\
+    (
+       higher_layer_preds.send_request tr client req_meta_data.server req_meta_data.request (get_label tr req_meta_data.key) /\
+      higher_layer_preds.send_response tr req_meta_data.server req_meta_data.request response key_label
+    ) \/ (
+      is_corrupt tr (principal_label client) \/ is_corrupt tr (principal_label req_meta_data.server)
     )
+  with _. (
+    let j = find_event_triggered_at_timestamp tr req_meta_data.server send_event in
+    higher_layer_preds.send_response_later (prefix tr j) tr req_meta_data.server req_meta_data.request response key_label;
+    ()
   )
   and _. ()
